fileSystem: specifications improved

fileSystem/theories/Spec/State.v
@@ -1,12 +1,93 @@
 Require Import BinInt.
 Require Import BinNat.
 Require Import Lia.
-Require Import FileSystem.
+Require Import Definitions.
 Require Import String.
 Require Import Ascii.
 Require Export Dec.
 
 Local Open Scope list.
+
+Inductive fileChar :=
+| Unknownc : fileChar
+| Nonec : fileChar
+| Somec : ascii -> fileChar.
+
+Definition funString := N -> fileChar.
+
+Record fdState : Type := MkFdState
+{
+	file : string;
+	mode : FileSystem.mode;
+	pos : N;
+}.
+
+Record fileState : Type := MkFileState
+{
+	size : option N;
+	content : funString;
+}.
+
+Record state : Type := MkState
+{
+	fds : Z -> option fdState;
+	files : string -> option fileState;
+}.
+
+Definition setFun {A B} (f : A -> B) (n : B) (i : A) `{forall (b : A), Decidable (i = b)} : A -> B :=
+fun (j : A) => if (# (i = j)) then n else f j.
+
+Lemma setFunOk {A B} (f : A -> B) (n : B) (i : A) `{forall (b : A), Decidable (i = b)}
+	: setFun f n i i = n.
+Proof.
+compute.
+destruct (H i).
+now destruct is_dec.
+Qed.
+
+Definition changeFun {A B} (f : A -> B) (fn : B -> B) (i : A) `{forall (b : A), Decidable (i = b)} : A -> B :=
+fun (j : A) => if (# (i = j)) then fn (f j) else f j.
+
+Lemma changeFunOk {A B} (f : A -> B) (fn : B -> B) (i : A) `{forall (b : A), Decidable (i = b)}
+	: changeFun f fn i i = fn (f i).
+Proof.
+compute.
+destruct (H i).
+now destruct is_dec.
+Qed.
+
+Fixpoint addString (s : string) (p : N) (c : funString) : funString :=
+	match s with
+	| String n ns => addString ns (p + 1) (setFun c (Somec n) p)
+	| _ => c
+	end.
+
+Fixpoint getString_aux (n : nat) (p : N) (c : funString) (acc : string) : option string :=
+	match n with
+	| S m => match c p with
+		|	Somec ch => getString_aux m (p + 1) c (acc ++ String ch "")
+		|	_ => None
+		end
+	| _ => Some acc
+	end.
+
+Definition getString (n : N) (p : N) (c : funString) : option string :=
+	getString_aux (N.to_nat n) p c "".
+
+Definition setFile (f : string -> string) (s : fdState) :=
+	let (a, b, c) := s in MkFdState (f a) b c.
+Definition setMode (f : FileSystem.mode -> FileSystem.mode) (s : fdState) :=
+	let (a, b, c) := s in MkFdState a (f b) c.
+Definition setPos (f : N -> N) (s : fdState) :=
+	let (a, b, c) := s in MkFdState a b (f c).
+
+Definition setSize (f : option N -> option N) (s : fileState) :=
+	let (a, b) := s in MkFileState (f a) b.
+Definition setContent (f : funString -> funString) (s : fileState) :=
+	let (a, b) := s in MkFileState a (f b).
+
+(*
+-----
 
 Definition partial (A B : Type) := A -> option B.
 
@@ -76,3 +157,5 @@ Definition setContent (f : fdContent -> fdContent) (s : fdState) :=
 	let (a, b, c, d, e) := s in MkFdState a b c d (f e).
 
 Definition state := partial Z fdState.
+
+*)
