fileSystem/theories/Spec/Post.v
@@ -1,9 +1,9 @@
-Require Import StateFun.
-Require Import FileSystem.
+Require Import State.
+Require Import Definitions.
 Require Import BinInt.
 Require Import String.
-
-Definition closed_fd (s : state) (fd : Z) : Prop := s fd = None.
+Require Import Props.
+Require Import Step.
 
 Definition rm_opt {A} (a : option (option A)) : option A :=
 	match a with
@@ -11,33 +11,32 @@ Definition rm_opt {A} (a : option (option A)) : option A :=
 	| None => None
 	end.
 
-Definition getPfun {A B C} (f : partial A B) (fe : B -> C) (i : A)
+Definition getPfun {A B C} (f : A -> option B) (fe : B -> C) (i : A)
 	:= option_map fe (f i).
 
-Definition getOpfun {A B C} (f : partial A B) (fe : B -> option C) (i : A)
+Definition getOpfun {A B C} (f : A -> option B) (fe : B -> option C) (i : A)
 	:= rm_opt (option_map fe (f i)).
 
 Inductive post : forall {A}, FileSystem.i A -> A -> state -> Prop :=
 (* Open returns a new file descriptor *)
 |	open_post (s : state) : forall (m : FileSystem.mode) (o : FileSystem.options)
-		(str : string) (fd : Z), closed_fd s fd -> post (FileSystem.Open m o str) fd s
-(* If kind or size are known, fstats returns them *)
+		(str : string) (fd : Z), ~ opened_fd s fd -> post (FileSystem.Open m o str) fd s
+(* If size is known, fstats returns it *)
 |	fstat_post (s : state) : forall (fd : Z)
 		(stats : FileSystem.stats),
-		(exists asize : N, getOpfun s size fd = Some asize -> asize = FileSystem.size stats) ->
-		(exists akind : FileSystem.fileKind, getOpfun s kind fd = Some akind -> akind = FileSystem.kind stats) ->
+		(* (exists asize : N, getOpfun s size fd = Some asize -> asize = FileSystem.size stats) -> *)
 		post (FileSystem.FStat fd) stats s
 (* If the size is known, getSize returns it *)
 |	getSize_post (s : state) : forall (fd : Z)
 		(psize : N),
-		(exists asize : N, getOpfun s size fd = Some asize -> asize = psize) ->
+		(* (exists asize : N, getOpfun s size fd = Some asize -> asize = psize) -> *)
 		post (FileSystem.GetSize fd) psize s
-(* If we know the position and the content of read area the file,
-		the returned string contains the content. *)
+(* If we know the content of read area the file,
+		the returned string contains this content. *)
 |	read_post (s : state) : forall (n : N) (fd : Z)
-		(pbuf : string) (ppos : N),
-		((exists apos : N, getOpfun s pos fd = Some apos -> apos = ppos) ->
-			(exists abuf : string, rm_opt (option_map (getString n ppos) (getPfun s content fd)) = Some abuf -> abuf = pbuf)) ->
+		(pbuf : string),
+		let p := getFilePos s fd in
+		(exists abuf : string, getString n p (getFileContent s fd) = Some abuf -> abuf = pbuf) ->
 				post (FileSystem.Read n fd) pbuf s
 |	write_post (s : state) : forall (str : string) (fd : Z),
 		post (FileSystem.Write str fd) tt s
