fileSystem/theories/Spec/Pre.v
@@ -1,0 +1,28 @@
+Require Import State.
+Require Import Definitions.
+Require Import BinInt.
+Require Import BinNat.
+Require Import String.
+Require Import Props.
+
+Inductive pre : forall {A}, FileSystem.i A -> state -> Prop :=
+|	open_pre (s : state) : forall (m : FileSystem.mode)
+		(o : FileSystem.options) (str : string)
+		(* We require that this file is not already opened *)
+		(Hno : ~(opened_file s str)),
+		pre (FileSystem.Open m o str) s
+| fstat_pre (s : state) : forall (fd : Z) (Ho : (opened_fd s fd)),
+		pre (FileSystem.FStat fd) s
+| getSize_pre (s : state) : forall (fd : Z) (Ho : (opened_fd s fd)),
+		pre (FileSystem.GetSize fd) s
+| read_pre (s : state) : forall (n : N) (fd : Z) (Ho : (opened_fd s fd)),
+		pre (FileSystem.Read n fd) s
+| write_pre (s : state) : forall (fd : Z) (str : string) (Ho : (opened_fd s fd)),
+		pre (FileSystem.Write str fd) s
+| seek_pre (s : state) : forall (fd n : Z) (ref : FileSystem.seekRef)
+		(Ho : (opened_fd s fd)),
+		pre (FileSystem.Seek ref n fd) s
+| close_pre (s : state) : forall (fd : Z) (Ho : (opened_fd s fd)),
+		pre (FileSystem.Close fd) s
+| unlink_pre (s : state) : forall (str : string), pre (FileSystem.Unlink str) s.
+
