fileSystem/theories/Spec/Props.v
@@ -1,0 +1,37 @@
+Require Import Definitions.
+Require Import State.
+Require Import Step.
+Require Import BinNat.
+Require Import BinInt.
+Require Import String.
+
+Definition initialState := MkState (const None) (const None).
+
+Definition opened_fd (s : state) (fd : Z) : Prop :=
+	let (sfd, sfile) := s in
+	sfd fd <> None.
+Definition opened_file (s : state) (str : string) : Prop :=
+	let (sfd, sfile) := s in
+	exists (fd : Z), option_map file (sfd fd) = Some str.
+
+Definition fileContentKnown (s : fileState) : Prop
+	:= forall (n : N), content s n <> Unknownc.
+
+Definition sameFileContent (sStart sEnd : fileState) : Prop
+	:= fileContentKnown sStart
+		/\ forall (n : N), content sStart n = content sEnd n.
+
+Definition sameFileContents (sStart sEnd : state) : Prop
+	:= forall (str : string) (sStartf : fileState), files sStart str = Some sStartf
+		-> exists (sEndf : fileState), files sEnd str = Some sEndf /\ sameFileContent sStartf sEndf.
+
+Definition setFileContent (s : state) (str content : string) : state
+	:= let (sfd, sfile) := s in
+		 let sfile := setFun sfile
+			(Some
+				(MkFileState
+					(Some (N.of_nat (length content)))
+					(addString content 0%N (const Nonec))
+				)
+			) str in
+			MkState sfd sfile.
