fileSystem/theories/Spec/Spec.v
@@ -1,0 +1,24 @@
+Require Import Definitions.
+Require Import Step.
+Require Import Pre.
+Require Import Post.
+Require Export State.
+Require Export Props.
+
+Require Import FreeSpec.Specification.
+
+(******************************************************************************
+This specification need the following hypothesis :
+	- all the files opened by the program must not be
+	  opened by any other program during all the execution
+
+It requires that :
+	- files can be opened only once until the corresponding file
+	  descriptor is closed
+******************************************************************************)
+
+Definition specs: Specification state FileSystem.i :=
+	{| abstract_step := @abs_step
+	;  precondition := @pre
+	;  postcondition := @post |}.
+
