fileSystem/theories/Spec/Step.v
@@ -1,0 +1,150 @@
+Require Import BinInt.
+Require Import BinNat.
+Require Import Definitions.
+Require Import State.
+Require Import String.
+
+From Equations Require Import Equations.
+
+Definition const {A B} (e : B) : A -> B := fun _ => e.
+
+Definition rm_opt {A} (a : option (option A)) : option A :=
+	match a with
+	|	Some o => o
+	| None => None
+	end.
+
+Definition option_map2 {A B C} (f : A -> B -> C) (a : option A) (b : option B) :=
+	match a with
+	|	Some a => match b with
+		|	Some b => Some (f a b)
+		| _ => None
+		end
+	|	_ => None
+	end.
+
+Definition Z_fun_to_N_fun (f : Z -> Z) := fun z => Z.to_N (f z).
+
+Definition getFileName (s : state) (fd : Z) :=
+	let (sfd, _) := s in
+	match (option_map file (sfd fd)) with
+	| Some s => s
+	| _ => ""%string (* Impossible *)
+	end.
+
+Definition getFilePos (s : state) (fd : Z) :=
+	let (sfd, _) := s in
+	match (option_map pos (sfd fd)) with
+	| Some p => p
+	| _ => 0%N (* Impossible *)
+	end.
+
+Definition getFileContent (s : state) (fd : Z) :=
+	let (_, sfile) := s in
+	match (option_map content (sfile (getFileName s fd))) with
+	| Some c => c
+	| _ => const Unknownc (* Impossible *)
+	end.
+
+Equations abs_step {A}
+	(op : FileSystem.i A)
+	(x : A)
+	(s : state)
+	: state :=
+
+abs_step (FileSystem.Open m o str) fd s :=
+	let (sfd, sfile) := s in
+	(* An entry for the new fd is added with the name and mode of the opened file
+	   The position in the file is 0 when it is opened *)
+	let sfd := setFun sfd (Some (MkFdState str m 0)) fd in
+	let sfile := match o with
+	|	FileSystem.MayCreateTruncate
+	|	FileSystem.DontCreateTruncate
+	|	FileSystem.MustCreate =>
+		(* With the truncate flag, the content of the file is reset *)
+		setFun sfile (Some (MkFileState (Some 0%N) (const Nonec))) str
+	|	_ =>
+		(* In the other case, we don't have information about the file *)
+		setFun sfile (Some (MkFileState (None) (const Unknownc))) str
+	end in
+	MkState sfd sfile ;
+
+(* Calling fstat allows to know the size of the file *)
+abs_step (FileSystem.FStat fd) x s :=
+	let (sfd, sfile) := s in
+	let str := getFileName s fd in
+	let s := changeFun sfile (option_map (setSize (const (Some (FileSystem.size x))))) str in
+	MkState sfd sfile ;
+
+(* Calling getSize allows to know the size of the file *)
+abs_step (FileSystem.GetSize fd) x s :=
+	let (sfd, sfile) := s in
+	let str := getFileName s fd in
+	let s := changeFun sfile (option_map (setSize (const (Some x)))) str in
+	MkState sfd sfile ;
+
+abs_step (FileSystem.Read n fd) x s :=
+	let (sfd, sfile) := s in
+	let str := getFileName s fd in
+	let p := getFilePos s fd in
+	(* The read text is in the file content *)
+	let sfile := changeFun sfile (option_map (setContent (addString x p))) str in
+	(* The position is updated after the read *)
+	let sfd := changeFun sfd (option_map (setPos (N.add (N.of_nat (length x))))) fd in
+	MkState sfd sfile ;
+
+abs_step (FileSystem.Write str fd) x s :=
+	let (sfd, sfile) := s in
+	let str := getFileName s fd in
+	let p := getFilePos s fd in
+	(* The written text is in the file content *)
+	let sfile := changeFun sfile (option_map (setContent (addString str p))) str in
+	(* The position is updated after the write *)
+	let sfd := changeFun sfd (option_map (setPos (N.add (N.of_nat (length str))))) fd in
+	(* If size < position, the file has been extended. The new size is the
+		new position *)
+	let p := getFilePos s fd in (* We get the updated position *)
+	let si := rm_opt (option_map size (sfile str)) in (* and the size, which may be unknown *)
+	let sfile := match (option_map (N.compare p) si) with
+	| Some LT =>
+		changeFun sfile (option_map (setSize (const (Some p)))) str
+	| _ =>
+		sfile
+	end in
+	MkState sfd sfile ;
+
+abs_step (FileSystem.Close fd) x s :=
+	let (sfd, sfile) := s in
+	(* The fd is now closed *)
+	let sfd := setFun sfd None fd in
+	MkState sfd sfile ;
+
+abs_step (FileSystem.Unlink str) x s :=
+	let (sfd, sfile) := s in
+	(* The file is removed *)
+	let sfile := setFun sfile None str in
+	MkState sfd sfile ;
+
+abs_step _ _ _ := s.
+
+Global Transparent abs_step.
+
+(* TODO Update
+abs_step (FileSystem.Seek ref n fd) x s :=
+	(* The position is updated *)
+	match ref with
+	| FileSystem.Beginning =>
+		let s := changeFun s (option_map (setPos (const (Some (Z.to_N n))))) fd in
+		s
+	| FileSystem.Current =>
+	(* If we know the previous position, we can compute the new position *)
+		let s := changeFun s (option_map (setPos (option_map (fun x => Z.to_N (Z.add n (Z.of_N x)))))) fd in
+		s
+	| FileSystem.End =>
+	(* If we know the size of the file, we can compute the new position *)
+		let size := rm_opt (option_map size (s fd)) in
+		let pos := option_map (fun x => Z.to_N (Z.add n (Z.of_N x))) size in
+		let s := changeFun s (option_map (setPos (const pos))) fd in
+		s
+	end ;
+*)
